src/lowparse/LowParseExample.fst
@@ -34,6 +34,12 @@ let j (input: FStar.Bytes.bytes) : Tot (option (LowParse.SLow.vlarray LowParseEx
 let m (x: LowParseExample.Aux.t) : Tot FStar.Bytes.bytes =
   LowParseExample.Aux.serialize32_t x
 
+// For now, extract the validator for compilation purposes only
+let v (x: LowStar.Buffer.buffer FStar.UInt8.t) (len: FStar.Int32.t) : FStar.HyperStack.ST.Stack FStar.Int32.t
+  (requires (fun _ -> False))
+  (ensures (fun _ _ _ -> True))
+= LowParseExample.Aux.validate32_t x len
+
 (*
 let msz ( x: LowParseExample.Aux.t) : Tot FStar.UInt32.t =
   LowParseExample.Aux.size32_t x
